checking prog equivalence in terms of local variable renamings. The renaming is manually from renaming.db.
git-svn-id: https://webdav.seas.upenn.edu/svn/sol/vol@2828 eef5ea85-cc2e-0410-bd84-0fae1f012da8

src/TV/sub_tv.v
@@ -18,7 +18,7 @@ Require Import Coq.Bool.Sumbool.
 
 Export SimpleSE.
 
-Definition tv_value (v v':value) := sumbool2bool _ _ (value_dec v v').
+Definition eq_value (v v':value) := sumbool2bool _ _ (value_dec v v').
 Definition tv_typ (t t':typ) := sumbool2bool _ _ (typ_dec t t').
 Definition tv_align (a a':align) := sumbool2bool _ _ (Align.dec a a').
 Definition eq_sterm (st st':sterm) := sumbool2bool _ _ (sterm_dec st st').
@@ -69,198 +69,12 @@ Axiom INT_is_one : INT -> bool.
 *)
 Axiom rename_fid : id -> id.
 
+(* In function f1, i1 is renamed to be (rename_id f1 i1) *)
+Axiom rename_id : id -> id -> id.
+
 Definition beps := list (id * id * id).
 Definition lbeps := list (l * beps).
 Definition flbeps := list (id * lbeps).
-
-(*
-declare weak void @__hashLoadBaseBound(
-  i8* %addr_of_ptr, 
-  i8** %addr_of_base, 
-  i8** %addr_of_bound, 
-  i8* %actual_ptr,    // useless 
-  i32 %size_of_type,  // useless
-  i32* %ptr_safe      // useless
-  )
-
-We assume 
-  1) We have already checked that %addr_of_base, %addr_of_bound and %ptr_safe 
-     are valid when being passed into @__hashLoadBaseBound. 
-    FIXME: Checking if they equal to "alloca..." 
-
-  2) __hashLoadBaseBound does not change %base, %bound and %ptr_safe.
-
-So, %base, %bound and %ptr_safe are safe to load w/o memsafety checks.
-*)
-Fixpoint load_from_metadata (sm:smem) (st:sterm) : bool :=
-match sm with
-| smem_init => false
-| smem_malloc sm1 _ _ _
-| smem_alloca sm1 _ _ _
-| smem_free sm1 _ _
-| smem_load sm1 _ _ _
-| smem_store sm1 _ _ _ _ => load_from_metadata sm1 st
-| smem_lib sm1 fid1 sts1 =>
-  if (is_hashLoadBaseBound fid1) then
-    match sts1 with
-    |  Cons_list_sterm _ 
-      (Cons_list_sterm addr_of_base
-      (Cons_list_sterm addr_of_bound
-      (Cons_list_sterm _
-      (Cons_list_sterm _
-      (Cons_list_sterm ptr_safe Nil_list_sterm))))) =>
-      if (eq_sterm st addr_of_base || 
-          eq_sterm st addr_of_bound || 
-          eq_sterm st ptr_safe) 
-      then true 
-      else load_from_metadata sm1 st
-    | _ => load_from_metadata sm1 st
-    end
-  else load_from_metadata sm1 st
-end.
-
-Fixpoint tv_sterm (st st':sterm) : bool :=
-match (st, st') with
-| (sterm_val v, sterm_val v') => tv_value v v'
-| (sterm_bop b sz st1 st2, sterm_bop b' sz' st1' st2') =>
-  sumbool2bool _ _ (bop_dec b b') && sumbool2bool _ _ (Size.dec sz sz') &&
-  tv_sterm st1 st1' && tv_sterm st2 st2'
-| (sterm_fbop b f st1 st2, sterm_fbop b' f' st1' st2') =>
-  sumbool2bool _ _ (fbop_dec b b') && 
-  sumbool2bool _ _ (floating_point_dec f f') &&
-  tv_sterm st1 st1' && tv_sterm st2 st2'
-| (sterm_extractvalue t st1 cs, sterm_extractvalue t' st1' cs') =>
-  tv_typ t t' && tv_sterm st1 st1' &&
-  sumbool2bool _ _ (list_const_dec cs cs')
-| (sterm_insertvalue t1 st1 t2 st2 cs, 
-   sterm_insertvalue t1' st1' t2' st2' cs') =>
-  tv_typ t1 t1' && tv_sterm st1 st1' && tv_typ t2 t2' && tv_sterm st2 st2' &&
-  sumbool2bool _ _ (list_const_dec cs cs')
-| (sterm_malloc sm t st1 a, sterm_malloc sm' t' st1' a') =>
-  tv_smem sm sm' && tv_typ t t' && tv_sterm st1 st1' && tv_align a a'
-| (sterm_alloca sm t st1 a, sterm_alloca sm' t' st1' a') =>
-  tv_smem sm sm' && tv_typ t t' && tv_sterm st1 st1' && tv_align a a'
-| (sterm_load sm t st1 a, sterm_load sm' t' st1' a') =>
-  tv_smem sm sm' && tv_typ t t' && tv_sterm st1 st1' && tv_align a a'
-| (sterm_gep i t st1 sts2, sterm_gep i' t' st1' sts2') =>
-  sumbool2bool _ _ (bool_dec i i') && tv_typ t t' &&
-  tv_sterm st1 st1' && tv_list_sterm sts2 sts2'
-| (sterm_trunc top t1 st1 t2, sterm_trunc top' t1' st1' t2') =>
-  sumbool2bool _ _ (truncop_dec top top') && tv_typ t1 t1' &&
-  tv_sterm st1 st1' && tv_typ t2 t2'
-| (sterm_ext eo t1 st1 t2, sterm_ext eo' t1' st1' t2') =>
-  sumbool2bool _ _ (extop_dec eo eo') && tv_typ t1 t1' &&
-  tv_sterm st1 st1' && tv_typ t2 t2' 
-| (sterm_cast co t1 st1 t2, sterm_cast co' t1' st1' t2') =>
-  sumbool2bool _ _ (castop_dec co co') && tv_typ t1 t1' &&
-  tv_sterm st1 st1' && tv_typ t2 t2' 
-| (sterm_icmp c t st1 st2, sterm_icmp c' t' st1' st2') =>
-  sumbool2bool _ _ (cond_dec c c') && tv_typ t t' &&
-  tv_sterm st1 st1' && tv_sterm st2 st2'
-| (sterm_fcmp c ft st1 st2, sterm_fcmp c' ft' st1' st2') =>
-  sumbool2bool _ _ (fcond_dec c c') &&
-  sumbool2bool _ _ (floating_point_dec ft ft') &&
-  tv_sterm st1 st1' && tv_sterm st2 st2'
-| (sterm_phi t stls, sterm_phi t' stls') =>
-  tv_typ t t' && tv_list_sterm_l stls stls'
-| (sterm_select st1 t st2 st3, sterm_select st1' t' st2' st3') =>
-  tv_sterm st1 st1' && tv_typ t t' && tv_sterm st2 st2' && tv_sterm st3 st3'
-| (sterm_lib sm i sts, sterm_lib sm' i' sts') =>
-  tv_smem sm sm' && eq_id i i' && tv_list_sterm sts sts'
-| _ => false
-end
-with tv_list_sterm (sts sts':list_sterm) : bool :=
-match (sts, sts') with
-| (Nil_list_sterm, Nil_list_sterm) => true
-| (Cons_list_sterm st sts0, Cons_list_sterm st' sts0') =>
-  tv_sterm st st' && tv_list_sterm sts0 sts0'
-| _ => false
-end
-with tv_list_sterm_l (stls stls':list_sterm_l) : bool :=
-match (stls, stls') with
-| (Nil_list_sterm_l, Nil_list_sterm_l) => true
-| (Cons_list_sterm_l st l stls0, Cons_list_sterm_l st' l' stls0') =>
-  tv_sterm st st' && sumbool2bool _ _ (l_dec l l') && 
-  tv_list_sterm_l stls0 stls0'
-| _ => false
-end
-with tv_smem (sm1 sm2:smem) : bool :=
-match (sm1, sm2) with
-| (smem_init, _) => true
-| (smem_malloc sm1 t1 st1 a1, smem_malloc sm2 t2 st2 a2) =>
-    tv_smem sm1 sm2 && tv_typ t1 t2 && tv_sterm st1 st2 && tv_align a1 a2
-| (smem_alloca sm1 t1 st1 a1, smem_alloca sm2 t2 st2 a2) =>
-    if (tv_typ t1 t2 && tv_sterm st1 st2 && tv_align a1 a2)
-    then tv_smem sm1 sm2
-    else tv_smem (smem_alloca sm1 t1 st1 a1) sm2
-| (smem_free sm1 t1 st1, smem_free sm2 t2 st2) =>
-    tv_smem sm1 sm2 && tv_typ t1 t2 && tv_sterm st1 st2
-| (smem_load sm1 t1 st1 a1, smem_load sm2 t2 st2 a2) =>
-    if (tv_typ t1 t2 && tv_sterm st1 st2 && tv_align a1 a2)
-    then tv_smem sm1 sm2
-    else tv_smem (smem_load sm1 t1 st1 a1) sm2
-| (smem_store sm1 t1 st11 st12 a1, smem_store sm2 t2 st21 st22 a2) =>
-    tv_smem sm1 sm2 && tv_typ t1 t2 && tv_sterm st11 st21 &&
-    tv_sterm st12 st22 && tv_align a1 a2
-| (smem_lib sm1 fid1 sts1, smem_lib sm2 fid2 sts2) => 
-    if (eq_id fid1 fid2 && tv_list_sterm sts1 sts2)
-    then tv_smem sm1 sm2
-    else tv_smem (smem_lib sm1 fid1 sts1) sm2
-| (sm1, smem_lib sm2 fid sts) => smem_lib_sub fid && tv_smem sm1 sm2
-| (sm1, smem_alloca sm2 t2 st2 a2) => tv_smem sm1 sm2
-| (sm1, smem_load sm2 t2 st2 a2) => 
-  (* We check load_from_metadata to ensure that the behavior of output programs 
-   * preserves input's. If we did not check, the additional load may be stuck. 
-   *)
-  tv_smem sm1 sm2 && load_from_metadata sm2 st2
-| _ => false
-end.
-
-Fixpoint tv_sframe (sf1 sf2:sframe) : bool :=
-match (sf1, sf2) with
-| (sframe_init, _) => true
-| (sframe_alloca sm1 sf1 t1 st1 a1, sframe_alloca sm2 sf2 t2 st2 a2) =>
-    if (tv_smem sm1 sm2 && tv_typ t1 t2 && tv_sterm st1 st2 && tv_align a1 a2)
-    then tv_sframe sf1 sf2
-    else tv_sframe (sframe_alloca sm1 sf1 t1 st1 a1) sf2
-| _ => false
-end.
-
-Fixpoint tv_smap (sm1 sm2:smap) : bool :=
-match sm1 with
-| nil => true
-| (id1,st1)::sm1' =>
-  match lookupAL _ sm2 id1 with
-  | None => false
-  | Some st2 => tv_sterm st1 st2 && tv_smap sm1' sm2
-  end
-end.
-
-Definition sub_sstate s1 s2 := 
-  tv_smap s1.(STerms) s2.(STerms) = true /\ 
-  tv_smem s1.(SMem) s2.(SMem) = true /\
-  tv_sframe s1.(SFrame) s2.(SFrame) = true /\ s1.(SEffects) = s2.(SEffects).
-
-Notation "s1 <<= s2" := (sub_sstate s1 s2) (at level 70, no associativity).
-
-Lemma sstate_sub_dec : forall (sts1 sts2:sstate), 
-  uniq sts1.(STerms) -> {sts1<<=sts2} + {~sts1<<=sts2}.
-Proof.
-Ltac done_right' := 
-  right; intro J ; destruct J as [ J1 [J2 [J3 J4]]]; simpl in *; auto.
-
-  intros sts1 sts2 Huniq.
-  destruct sts1 as [st1 sm1 sf1 se1].
-  destruct sts2 as [st2 sm2 sf2 se2].
-  destruct (@sterms_dec se1 se2); subst; try solve [done_right'].
-  unfold sub_sstate. simpl.
-  destruct (tv_smap st1 st2); auto.
-  destruct (tv_smem sm1 sm2); auto.
-  destruct (tv_sframe sf1 sf2); auto.
-    right. intro J ; destruct J as [ J1 [J2 [J3 J4]]]. inversion J3.
-    right. intro J ; destruct J as [ J1 [J2 [J3 J4]]]. inversion J2.
-    right. intro J ; destruct J as [ J1 [J2 [J3 J4]]]. inversion J1.
-Qed.
 
 (* cast does not change value. We can prove they have the same operational
  * semantics. *)
@@ -291,23 +105,6 @@ end.
 
 Definition eq_sterm_upto_cast (st1 st2:sterm) : bool :=
 eq_sterm (remove_cast st1) (remove_cast st2).
-
-Fixpoint is_addrof_be_aux (abes:list (id*id*id)) (fid ab ae:id)
-  : bool :=
-match abes with
-| nil => false
-| (fid', ab', ae')::abes' => 
-    if (eq_id fid fid' && eq_id ab ab' && eq_id ae ae') then true
-    else is_addrof_be_aux abes' fid ab ae
-end.
-
-Definition is_addrof_be (fid:id) (sab sae:sterm) : bool :=
-match (sab, sae) with
-| (sterm_val (value_id ab), sterm_val (value_id ae)) =>
-  is_addrof_be_aux (get_addrof_be tt) fid ab ae
-| (sterm_alloca _ _ _ _, sterm_alloca _ _ _ _) => true
-| _ => false
-end.
 
 (************************************************************)
 (* Generating metadata *) 
@@ -719,7 +516,394 @@ match m2 with
 | module_intro _ _ Ps2 => addrofbe_from_products Ps2 nil
 end.
 
-(************************************************************)
+(***********************************************)
+(* Sub TV *)
+
+(*
+declare weak void @__hashLoadBaseBound(
+  i8* %addr_of_ptr, 
+  i8** %addr_of_base, 
+  i8** %addr_of_bound, 
+  i8* %actual_ptr,    // useless 
+  i32 %size_of_type,  // useless
+  i32* %ptr_safe      // useless
+  )
+
+We assume 
+  1) We have already checked that %addr_of_base, %addr_of_bound and %ptr_safe 
+     are valid when being passed into @__hashLoadBaseBound. 
+    FIXME: Checking if they equal to "alloca..." 
+
+  2) __hashLoadBaseBound does not change %base, %bound and %ptr_safe.
+
+So, %base, %bound and %ptr_safe are safe to load w/o memsafety checks.
+*)
+Fixpoint load_from_metadata (sm:smem) (st:sterm) : bool :=
+match sm with
+| smem_init => false
+| smem_malloc sm1 _ _ _
+| smem_alloca sm1 _ _ _
+| smem_free sm1 _ _
+| smem_load sm1 _ _ _
+| smem_store sm1 _ _ _ _ => load_from_metadata sm1 st
+| smem_lib sm1 fid1 sts1 =>
+  if (is_hashLoadBaseBound fid1) then
+    match sts1 with
+    |  Cons_list_sterm _ 
+      (Cons_list_sterm addr_of_base
+      (Cons_list_sterm addr_of_bound
+      (Cons_list_sterm _
+      (Cons_list_sterm _
+      (Cons_list_sterm ptr_safe Nil_list_sterm))))) =>
+      if (eq_sterm st addr_of_base || 
+          eq_sterm st addr_of_bound || 
+          eq_sterm st ptr_safe) 
+      then true 
+      else load_from_metadata sm1 st
+    | _ => load_from_metadata sm1 st
+    end
+  else load_from_metadata sm1 st
+end.
+
+Definition tv_id fid (id1 id2:id) : bool :=
+  eq_id (rename_id fid id1) id2.
+
+Axiom tv_id_injective1 : forall fid id1 id2 id1' id2',
+  id1 = id2 -> tv_id fid id1 id1' -> tv_id fid id2 id2' -> id1' = id2'.
+
+Axiom tv_id_injective2 : forall fid id1 id2 id1' id2',
+  id1 <> id2 -> tv_id fid id1 id1' -> tv_id fid id2 id2' -> id1' <> id2'.
+
+Definition tv_value fid v1 v2 : bool :=
+match (v1, v2) with
+| (value_id id1, value_id id2) => tv_id fid id1 id2
+| (v1, v2) => eq_value v1 v2
+end.
+
+Fixpoint tv_sterm fid (st st':sterm) : bool :=
+match (st, st') with
+| (sterm_val v, sterm_val v') => tv_value fid v v'
+| (sterm_bop b sz st1 st2, sterm_bop b' sz' st1' st2') =>
+    sumbool2bool _ _ (bop_dec b b') && sumbool2bool _ _ (Size.dec sz sz') &&
+    tv_sterm fid st1 st1' && tv_sterm fid st2 st2'
+| (sterm_fbop b f st1 st2, sterm_fbop b' f' st1' st2') =>
+    sumbool2bool _ _ (fbop_dec b b') && 
+    sumbool2bool _ _ (floating_point_dec f f') &&
+    tv_sterm fid st1 st1' && tv_sterm fid st2 st2'
+| (sterm_extractvalue t st1 cs, sterm_extractvalue t' st1' cs') =>
+    tv_typ t t' && tv_sterm fid st1 st1' &&
+  sumbool2bool _ _ (list_const_dec cs cs')
+| (sterm_insertvalue t1 st1 t2 st2 cs, 
+   sterm_insertvalue t1' st1' t2' st2' cs') =>
+    tv_typ t1 t1' && tv_sterm fid st1 st1' && 
+    tv_typ t2 t2' && tv_sterm fid st2 st2' &&
+    sumbool2bool _ _ (list_const_dec cs cs')
+| (sterm_malloc sm t st1 a, sterm_malloc sm' t' st1' a') =>
+    tv_smem fid sm sm' && tv_typ t t' && tv_sterm fid st1 st1' && tv_align a a'
+| (sterm_alloca sm t st1 a, sterm_alloca sm' t' st1' a') =>
+    tv_smem fid sm sm' && tv_typ t t' && tv_sterm fid st1 st1' && tv_align a a'
+| (sterm_load sm t st1 a, sterm_load sm' t' st1' a') =>
+    tv_smem fid sm sm' && tv_typ t t' && tv_sterm fid st1 st1' && tv_align a a'
+| (sterm_gep i t st1 sts2, sterm_gep i' t' st1' sts2') =>
+    sumbool2bool _ _ (bool_dec i i') && tv_typ t t' &&
+    tv_sterm fid st1 st1' && tv_list_sterm fid sts2 sts2'
+| (sterm_trunc top t1 st1 t2, sterm_trunc top' t1' st1' t2') =>
+    sumbool2bool _ _ (truncop_dec top top') && tv_typ t1 t1' &&
+    tv_sterm fid st1 st1' && tv_typ t2 t2'
+| (sterm_ext eo t1 st1 t2, sterm_ext eo' t1' st1' t2') =>
+    sumbool2bool _ _ (extop_dec eo eo') && tv_typ t1 t1' &&
+    tv_sterm fid st1 st1' && tv_typ t2 t2' 
+| (sterm_cast co t1 st1 t2, sterm_cast co' t1' st1' t2') =>
+    sumbool2bool _ _ (castop_dec co co') && tv_typ t1 t1' &&
+    tv_sterm fid st1 st1' && tv_typ t2 t2' 
+| (sterm_icmp c t st1 st2, sterm_icmp c' t' st1' st2') =>
+    sumbool2bool _ _ (cond_dec c c') && tv_typ t t' &&
+    tv_sterm fid st1 st1' && tv_sterm fid st2 st2'
+| (sterm_fcmp c ft st1 st2, sterm_fcmp c' ft' st1' st2') =>
+    sumbool2bool _ _ (fcond_dec c c') &&
+    sumbool2bool _ _ (floating_point_dec ft ft') &&
+    tv_sterm fid st1 st1' && tv_sterm fid st2 st2'
+| (sterm_phi t stls, sterm_phi t' stls') =>
+    tv_typ t t' && tv_list_sterm_l fid stls stls'
+| (sterm_select st1 t st2 st3, sterm_select st1' t' st2' st3') =>
+    tv_sterm fid st1 st1' && tv_typ t t' && 
+    tv_sterm fid st2 st2' && tv_sterm fid st3 st3'
+| (sterm_lib sm i sts, sterm_lib sm' i' sts') =>
+    tv_smem fid sm sm' && eq_id i i' && tv_list_sterm fid sts sts'
+| _ => false
+end
+with tv_list_sterm fid (sts sts':list_sterm) : bool :=
+match (sts, sts') with
+| (Nil_list_sterm, Nil_list_sterm) => true
+| (Cons_list_sterm st sts0, Cons_list_sterm st' sts0') =>
+    tv_sterm fid st st' && tv_list_sterm fid sts0 sts0'
+| _ => false
+end
+with tv_list_sterm_l fid (stls stls':list_sterm_l) : bool :=
+match (stls, stls') with
+| (Nil_list_sterm_l, Nil_list_sterm_l) => true
+| (Cons_list_sterm_l st l stls0, Cons_list_sterm_l st' l' stls0') =>
+    tv_sterm fid st st' && sumbool2bool _ _ (l_dec l l') && 
+    tv_list_sterm_l fid stls0 stls0'
+| _ => false
+end
+with tv_smem fid (sm1 sm2:smem) : bool :=
+match (sm1, sm2) with
+| (smem_init, _) => true
+| (smem_malloc sm1 t1 st1 a1, smem_malloc sm2 t2 st2 a2) =>
+    tv_smem fid sm1 sm2 && tv_typ t1 t2 && tv_sterm fid st1 st2 && tv_align a1 a2
+| (smem_alloca sm1 t1 st1 a1, smem_alloca sm2 t2 st2 a2) =>
+    if (tv_typ t1 t2 && tv_sterm fid st1 st2 && tv_align a1 a2)
+    then tv_smem fid sm1 sm2
+    else tv_smem fid (smem_alloca sm1 t1 st1 a1) sm2
+| (smem_free sm1 t1 st1, smem_free sm2 t2 st2) =>
+    tv_smem fid sm1 sm2 && tv_typ t1 t2 && tv_sterm fid st1 st2
+| (smem_load sm1 t1 st1 a1, smem_load sm2 t2 st2 a2) =>
+    if (tv_typ t1 t2 && tv_sterm fid st1 st2 && tv_align a1 a2)
+    then tv_smem fid sm1 sm2
+    else tv_smem fid (smem_load sm1 t1 st1 a1) sm2
+| (smem_store sm1 t1 st11 st12 a1, smem_store sm2 t2 st21 st22 a2) =>
+    tv_smem fid sm1 sm2 && tv_typ t1 t2 && tv_sterm fid st11 st21 &&
+    tv_sterm fid st12 st22 && tv_align a1 a2
+| (smem_lib sm1 fid1 sts1, smem_lib sm2 fid2 sts2) => 
+    if (eq_id fid1 fid2 && tv_list_sterm fid sts1 sts2)
+    then tv_smem fid sm1 sm2
+    else tv_smem fid (smem_lib sm1 fid1 sts1) sm2
+| (sm1, smem_lib sm2 fid sts) => smem_lib_sub fid && tv_smem fid sm1 sm2
+| (sm1, smem_alloca sm2 t2 st2 a2) => tv_smem fid sm1 sm2
+| (sm1, smem_load sm2 t2 st2 a2) => 
+  (* We check load_from_metadata to ensure that the behavior of output programs 
+   * preserves input's. If we did not check, the additional load may be stuck. 
+   *)
+    tv_smem fid sm1 sm2 && load_from_metadata sm2 st2
+| _ => false
+end.
+
+Fixpoint tv_sframe fid (sf1 sf2:sframe) : bool :=
+match (sf1, sf2) with
+| (sframe_init, _) => true
+| (sframe_alloca sm1 sf1 t1 st1 a1, sframe_alloca sm2 sf2 t2 st2 a2) =>
+    if (tv_smem fid sm1 sm2 && tv_typ t1 t2 && 
+        tv_sterm fid st1 st2 && tv_align a1 a2)
+    then tv_sframe fid sf1 sf2
+    else tv_sframe fid (sframe_alloca sm1 sf1 t1 st1 a1) sf2
+| _ => false
+end.
+
+Fixpoint tv_smap fid (sm1 sm2:smap) : bool :=
+match sm1 with
+| nil => true
+| (id1,st1)::sm1' =>
+  match lookupAL _ sm2 (rename_id fid id1) with
+  | None => false
+  | Some st2 => tv_sterm fid st1 st2 && tv_smap fid sm1' sm2
+  end
+end.
+
+Definition sub_sstate fid s1 s2 := 
+  tv_smap fid s1.(STerms) s2.(STerms) = true /\ 
+  tv_smem fid s1.(SMem) s2.(SMem) = true /\
+  tv_sframe fid s1.(SFrame) s2.(SFrame) = true /\ s1.(SEffects) = s2.(SEffects).
+
+Lemma sstate_sub_dec : forall fid (sts1 sts2:sstate), 
+  uniq sts1.(STerms) -> {sub_sstate fid sts1 sts2} + {~sub_sstate fid sts1 sts2}.
+Proof.
+Ltac done_right' := 
+  right; intro J ; destruct J as [ J1 [J2 [J3 J4]]]; simpl in *; auto.
+
+  intros fid sts1 sts2 Huniq.
+  destruct sts1 as [st1 sm1 sf1 se1].
+  destruct sts2 as [st2 sm2 sf2 se2].
+  destruct (@sterms_dec se1 se2); subst; try solve [done_right'].
+  unfold sub_sstate. simpl.
+  destruct (tv_smap fid st1 st2); auto.
+  destruct (tv_smem fid sm1 sm2); auto.
+  destruct (tv_sframe fid sf1 sf2); auto.
+    right. intro J ; destruct J as [ J1 [J2 [J3 J4]]]. inversion J3.
+    right. intro J ; destruct J as [ J1 [J2 [J3 J4]]]. inversion J2.
+    right. intro J ; destruct J as [ J1 [J2 [J3 J4]]]. inversion J1.
+Qed.
+
+Definition tv_cmds fid (nbs1 nbs2 : list nbranch) :=
+sumbool2bool _ _ 
+  (sstate_sub_dec fid 
+    (se_cmds sstate_init nbs1) 
+    (se_cmds sstate_init nbs2) 
+    (se_cmds_init_uniq nbs1)).
+
+(* Here, we check which function to call conservatively. In practice, a v1
+ * is a function pointer, we should look up the function name from the 
+ * FunTable. Since the LLVM IR takes function names as function pointers,
+ * if a program does not assign them to be other variables, they should
+ * be the same. *)
+Fixpoint tv_params fid (tsts1 tsts2:list (typ*sterm)) : bool :=
+match (tsts1, tsts2) with
+| (nil, _) => true
+| ((t1,st1)::tsts1', (t2,st2)::tsts2') => 
+  tv_typ t1 t2 && tv_sterm fid st1 st2 && tv_params fid tsts1' tsts2'
+| _ => false
+end.
+
+Definition tv_fid (fid1 fid2:id) := 
+  eq_id (rename_fid fid1) fid2.
+
+Axiom tv_fid_injective1 : forall fid1 fid2 fid1' fid2',
+  fid1 = fid2 -> tv_fid fid1 fid1' -> tv_fid fid2 fid2' -> fid1' = fid2'.
+
+Axiom tv_fid_injective2 : forall fid1 fid2 fid1' fid2',
+  fid1 <> fid2 -> tv_fid fid1 fid1' -> tv_fid fid2 fid2' -> fid1' <> fid2'.
+
+(* Do not check if their tailc flags match. Softbound changes the flag for
+ * system calls, say atoi from tailcall to non-tailcall.
+ *)
+Definition tv_scall fid (c1 c2:scall) :=
+  let '(stmn_call rid1 nr1 _ t1 v1 tsts1) := c1 in
+  let '(stmn_call rid2 nr2 _ t2 v2 tsts2) := c2 in
+  eq_id rid1 rid1 &&
+  (sumbool2bool _ _ (noret_dec nr1 nr2)) &&
+  tv_typ t1 t2 && tv_params fid tsts1 tsts2 &&
+  match (v1, v2) with
+  | (value_const (const_gid _ fid1), value_const (const_gid _ fid2)) => 
+      tv_fid fid1 fid2
+  | (v1, v2) => sumbool2bool _ _ (value_dec v1 v2)
+  end.
+
+Definition tv_subblock fid (sb1 sb2:subblock) :=
+match (sb1, sb2) with
+| (mkSB nbs1 call1 iscall1, mkSB nbs2 call2 iscall2) =>
+  let st1 := se_cmds sstate_init nbs1 in
+  let st2 := se_cmds sstate_init nbs2 in
+  let cl1 := se_call st1 call1 iscall1 in
+  let cl2 := se_call st2 call2 iscall2 in
+   (sumbool2bool _ _ (sstate_sub_dec fid st1 st2 (se_cmds_init_uniq nbs1)))
+end.
+
+Fixpoint tv_subblocks fid (sbs1 sbs2:list subblock) :=
+match (sbs1, sbs2) with
+| (nil, nil) => true
+| (sb1::sbs1', sb2::sbs2') => 
+    (tv_subblock fid sb1 sb2) && (tv_subblocks fid sbs1' sbs2')
+| _ => false
+end.
+
+Fixpoint tv_list_value_l fid (vls1 vls2:list_value_l) : bool :=
+match (vls1, vls2) with
+| (Nil_list_value_l, Nil_list_value_l) => true
+| (Cons_list_value_l v1 l1 vls1, Cons_list_value_l v2 l2 vls2) =>
+    tv_value fid v1 v2 && eq_l l1 l2 && tv_list_value_l fid vls1 vls2
+| _ => false
+end.
+
+Definition tv_phinode fid (p1 p2:phinode) : bool :=
+match (p1, p2) with
+| (insn_phi id1 t1 vls1, insn_phi id2 t2 vls2) =>
+    tv_id fid id1 id2  && tv_typ t1 t2 && tv_list_value_l fid vls1 vls2
+end.
+
+Fixpoint tv_phinodes fid (ps1 ps2:phinodes) : bool :=
+match ps1 with
+| nil => true
+| (insn_phi i1 _ _)as p1::ps1' =>
+  match lookupPhinode ps2 i1 with
+  | None => false
+  | Some p2 => tv_phinode fid p1 p2 && tv_phinodes fid ps1' ps2
+  end
+end.
+
+Definition tv_terminator fid (tmn1 tmn2:terminator) : bool :=
+match (tmn1, tmn2) with
+| (insn_return id1 t1 v1, insn_return id2 t2 v2) => 
+    tv_id fid id1 id2 && tv_typ t1 t2 && tv_value fid v1 v2
+| (insn_return_void id1, insn_return_void id2) => tv_id fid id1 id2
+| (insn_br id1 v1 l11 l12, insn_br id2 v2 l21 l22) =>
+    tv_id fid id1 id2 && tv_value fid v1 v2 && eq_l l11 l21 && eq_l l12 l22
+| (insn_br_uncond id1 l1, insn_br_uncond id2 l2) =>
+    tv_id fid id1 id2 && eq_l l1 l2
+| (insn_unreachable id1, insn_unreachable id2) => tv_id fid id1 id2
+| _ => false
+end.
+
+Definition tv_block fid (b1 b2:block) :=
+match (b1, b2) with
+| (block_intro l1 ps1 cs1 tmn1, block_intro l2 ps2 cs2 tmn2) =>
+  match (cmds2sbs cs1, cmds2sbs cs2) with
+  | ((sbs1, nbs1), (sbs2, nbs2)) =>
+    eq_l l1 l2 && tv_phinodes fid ps1 ps2 && tv_subblocks fid sbs1 sbs2 &&
+    tv_cmds fid nbs1 nbs2 && tv_terminator fid tmn1 tmn2
+  end
+end.
+
+Fixpoint tv_blocks fid (bs1 bs2:blocks):=
+match (bs1, bs2) with
+| (nil, nil) => true
+| (b1::bs1', b2::bs2') => tv_block fid b1 b2 && tv_blocks fid bs1' bs2'
+| _ => false
+end.
+
+Definition tv_fheader (f1 f2:fheader) := 
+  let '(fheader_intro t1 fid1 a1) := f1 in
+  let '(fheader_intro t2 fid2 a2) := f2 in
+  (sumbool2bool _ _ (typ_dec t1 t2)) &&
+  tv_fid fid1 fid2 &&
+  (sumbool2bool _ _ (prefix_dec _ arg_dec a1 a2)).
+
+Definition tv_fdec (f1 f2:fdec) :=
+match (f1, f2) with
+| (fdec_intro fh1, fdec_intro fh2) => tv_fheader fh1 fh2
+end.
+
+Definition tv_fdef (f1 f2:fdef) :=
+match (f1, f2) with
+| (fdef_intro (fheader_intro _ fid1 _ as fh1) lb1, fdef_intro fh2 lb2) =>
+  tv_fheader fh1 fh2 && tv_blocks fid1 lb1 lb2
+end.
+
+Fixpoint lookupGvarViaIDFromProducts (lp:products) (i:id) : option gvar :=
+match lp with
+| nil => None
+| (product_gvar gv)::lp' => 
+    if (eq_dec (getGvarID gv) i) then Some gv
+    else lookupGvarViaIDFromProducts lp' i
+| _::lp' => lookupGvarViaIDFromProducts lp' i
+end.
+
+Fixpoint tv_products (Ps1 Ps2:products) : bool :=
+match Ps1 with
+| nil => true
+| product_gvar gv1::Ps1' =>
+  match lookupGvarViaIDFromProducts Ps2 (getGvarID gv1) with
+  | None => false
+  | Some gv2 => sumbool2bool _ _ (gvar_dec gv1 gv2) && tv_products Ps1' Ps2 
+  end
+| product_fdec f1::Ps1' =>
+  match lookupFdecViaIDFromProducts Ps2 (rename_fid (getFdecID f1)) with
+  | None => false
+  | Some f2 => tv_fdec f1 f2 && tv_products Ps1' Ps2 
+  end
+| product_fdef f1::Ps1' =>
+  match lookupFdefViaIDFromProducts Ps2 (rename_fid (getFdefID f1)) with
+  | None => false
+  | Some f2 => tv_fdef f1 f2 && tv_products Ps1' Ps2 
+  end
+end.
+
+Definition tv_module (m1 m2:module) :=
+match (m1, m2) with
+| (module_intro los1 nts1 Ps1, module_intro los2 nts2 Ps2) =>
+  sumbool2bool _ _ (layouts_dec los1 los2) &&
+  sumbool2bool _ _ (namedts_dec nts1 nts2) &&
+  tv_products Ps1 Ps2
+end.
+
+Fixpoint tv_system (S1 S2:system) :=
+match (S1, S2) with
+| (nil, nil) => true
+| (m1::S1', m2::S2') => tv_module m1 m2 && tv_system S1' S2'
+| _ => false
+end.
+
+(*************************************)
+(* MTV *)
 
 (* 
    ptr = load addr_of_ptr
@@ -848,6 +1032,23 @@ if (is_hashLoadBaseBound lid) then
   | _ => false
   end      
 else true.
+
+Fixpoint is_addrof_be_aux (abes:list (id*id*id)) (fid ab ae:id)
+  : bool :=
+match abes with
+| nil => false
+| (fid', ab', ae')::abes' => 
+    if (eq_id fid fid' && eq_id ab ab' && eq_id ae ae') then true
+    else is_addrof_be_aux abes' fid ab ae
+end.
+
+Definition is_addrof_be (fid:id) (sab sae:sterm) : bool :=
+match (sab, sae) with
+| (sterm_val (value_id ab), sterm_val (value_id ae)) =>
+  is_addrof_be_aux (get_addrof_be tt) fid ab ae
+| (sterm_alloca _ _ _ _, sterm_alloca _ _ _ _) => true
+| _ => false
+end.
 
 (* ptr is safe to access if ptr is asserted by a deref check or
    from hasLoadBaseBound *)
@@ -1001,51 +1202,11 @@ end.
 Definition check_addrof_be fid sm :=
   check_addrof_be_aux fid sm (get_addrof_be tt).
 
-Definition tv_cmds (nbs1 nbs2 : list nbranch) :=
-sumbool2bool _ _ (sstate_sub_dec (se_cmds sstate_init nbs1) (se_cmds sstate_init nbs2) (se_cmds_init_uniq nbs1)).
-
 Definition mtv_cmds fid l (nbs2 : list nbranch) :=
 let st2 := se_cmds sstate_init nbs2 in 
 smem_is_memsafe fid l st2.(SMem) &&
 check_all_metadata fid l st2.(STerms) &&
 check_addrof_be fid st2.(STerms).
-
-(* Here, we check which function to call conservatively. In practice, a v1
- * is a function pointer, we should look up the function name from the 
- * FunTable. Since the LLVM IR takes function names as function pointers,
- * if a program does not assign them to be other variables, they should
- * be the same. *)
-Fixpoint tv_params (tsts1 tsts2:list (typ*sterm)) : bool :=
-match (tsts1, tsts2) with
-| (nil, _) => true
-| ((t1,st1)::tsts1', (t2,st2)::tsts2') => 
-  tv_typ t1 t2 && tv_sterm st1 st2 && tv_params tsts1' tsts2'
-| _ => false
-end.
-
-Definition tv_fid (fid1 fid2:id) := 
-  eq_id (rename_fid fid1) fid2.
-
-Axiom tv_fid_injective1 : forall fid1 fid2 fid1' fid2',
-  fid1 = fid2 -> tv_fid fid1 fid1' -> tv_fid fid2 fid2' -> fid1' = fid2'.
-
-Axiom tv_fid_injective2 : forall fid1 fid2 fid1' fid2',
-  fid1 <> fid2 -> tv_fid fid1 fid1' -> tv_fid fid2 fid2' -> fid1' <> fid2'.
-
-(* Do not check if their tailc flags match. Softbound changes the flag for
- * system calls, say atoi from tailcall to non-tailcall.
- *)
-Definition tv_scall (c1 c2:scall) :=
-  let '(stmn_call rid1 nr1 _ t1 v1 tsts1) := c1 in
-  let '(stmn_call rid2 nr2 _ t2 v2 tsts2) := c2 in
-  eq_id rid1 rid1 &&
-  (sumbool2bool _ _ (noret_dec nr1 nr2)) &&
-  tv_typ t1 t2 && tv_params tsts1 tsts2 &&
-  match (v1, v2) with
-  | (value_const (const_gid _ fid1), value_const (const_gid _ fid2)) => 
-      tv_fid fid1 fid2
-  | (v1, v2) => sumbool2bool _ _ (value_dec v1 v2)
-  end.
 
 (* We assume that the orders of ars and sars are matched. The function finds
    the corresponding sterm to arg with id i. *)
@@ -1095,16 +1256,6 @@ Definition mtv_scall Ps2 fid l1 (c2:scall) :=
   | _ => true
   end.
 
-Definition tv_subblock (sb1 sb2:subblock) :=
-match (sb1, sb2) with
-| (mkSB nbs1 call1 iscall1, mkSB nbs2 call2 iscall2) =>
-  let st1 := se_cmds sstate_init nbs1 in
-  let st2 := se_cmds sstate_init nbs2 in
-  let cl1 := se_call st1 call1 iscall1 in
-  let cl2 := se_call st2 call2 iscall2 in
-   (sumbool2bool _ _ (sstate_sub_dec st1 st2 (se_cmds_init_uniq nbs1)))
-end.
-
 Definition mtv_subblock Ps2 fid l (sb2:subblock) :=
 match sb2 with
 | mkSB nbs2 call2 iscall2 =>
@@ -1116,29 +1267,10 @@ match sb2 with
    mtv_scall Ps2 fid l cl2
 end.
 
-Fixpoint tv_subblocks (sbs1 sbs2:list subblock) :=
-match (sbs1, sbs2) with
-| (nil, nil) => true
-| (sb1::sbs1', sb2::sbs2') => 
-   (tv_subblock sb1 sb2) && (tv_subblocks sbs1' sbs2')
-| _ => false
-end.
-
 Fixpoint mtv_subblocks Ps2 fid l (sbs2:list subblock) :=
 match sbs2 with
 | nil => true
 | sb2::sbs2' => mtv_subblock Ps2 fid l sb2 && mtv_subblocks Ps2 fid l sbs2'
-end.
-
-Fixpoint tv_phinodes (ps1 ps2:phinodes) : bool :=
-match ps1 with
-| nil => true
-| (insn_phi i1 _ _)as p1::ps1' =>
-  match lookupPhinode ps2 i1 with
-  | None => false
-  | Some p2 => 
-    sumbool2bool _ _ (phinode_dec p1 p2) && tv_phinodes ps1' ps2
-  end
 end.
 
 (* Check
@@ -1190,19 +1322,6 @@ end.
 Definition mtv_phinodes fid l (ps2:phinodes) : bool :=
   mtv_phinodes_aux fid l (get_metadata tt) ps2.
 
-Definition tv_block (b1 b2:block) :=
-match (b1, b2) with
-| (block_intro l1 ps1 cs1 tmn1, block_intro l2 ps2 cs2 tmn2) =>
-  match (cmds2sbs cs1, cmds2sbs cs2) with
-  | ((sbs1, nbs1), (sbs2, nbs2)) =>
-    sumbool2bool _ _ (eq_atom_dec l1 l2) &&
-    tv_phinodes ps1 ps2 &&
-    tv_subblocks sbs1 sbs2 &&
-    tv_cmds nbs1 nbs2 &&
-    sumbool2bool _ _ (terminator_dec tmn1 tmn2)
-  end
-end.
-
 Definition mtv_block Ps2 fid (b2:block) :=
 match b2 with
 | block_intro l2 ps2 cs2 tmn2 =>
@@ -1213,70 +1332,16 @@ match b2 with
   end
 end.
 
-Fixpoint tv_blocks (bs1 bs2:blocks):=
-match (bs1, bs2) with
-| (nil, nil) => true
-| (b1::bs1', b2::bs2') => tv_block b1 b2 && tv_blocks bs1' bs2'
-| _ => false
-end.
-
 Fixpoint mtv_blocks Ps2 fid (bs2:blocks):=
 match bs2 with
 | nil => true
 | b2::bs2' => mtv_block Ps2 fid b2 && mtv_blocks Ps2 fid bs2'
 end.
 
-Definition tv_fheader (f1 f2:fheader) := 
-  let '(fheader_intro t1 fid1 a1) := f1 in
-  let '(fheader_intro t2 fid2 a2) := f2 in
-  (sumbool2bool _ _ (typ_dec t1 t2)) &&
-  tv_fid fid1 fid2 &&
-  (sumbool2bool _ _ (prefix_dec _ arg_dec a1 a2)).
-
-Definition tv_fdec (f1 f2:fdec) :=
-match (f1, f2) with
-| (fdec_intro fh1, fdec_intro fh2) => tv_fheader fh1 fh2
-end.
-
-Definition tv_fdef (f1 f2:fdef) :=
-match (f1, f2) with
-| (fdef_intro fh1 lb1, fdef_intro fh2 lb2) =>
-  tv_fheader fh1 fh2 && tv_blocks lb1 lb2
-end.
-
 Definition mtv_fdef Ps2 (f2:fdef) :=
 match f2 with
 | fdef_intro ((fheader_intro t2 fid2 a2) as fh2) lb2 =>
   if (isCallLib fid2) then true else mtv_blocks Ps2 fid2 lb2
-end.
-
-Fixpoint lookupGvarViaIDFromProducts (lp:products) (i:id) : option gvar :=
-match lp with
-| nil => None
-| (product_gvar gv)::lp' => 
-    if (eq_dec (getGvarID gv) i) then Some gv
-    else lookupGvarViaIDFromProducts lp' i
-| _::lp' => lookupGvarViaIDFromProducts lp' i
-end.
-
-Fixpoint tv_products (Ps1 Ps2:products) : bool :=
-match Ps1 with
-| nil => true
-| product_gvar gv1::Ps1' =>
-  match lookupGvarViaIDFromProducts Ps2 (getGvarID gv1) with
-  | None => false
-  | Some gv2 => sumbool2bool _ _ (gvar_dec gv1 gv2) && tv_products Ps1' Ps2 
-  end
-| product_fdec f1::Ps1' =>
-  match lookupFdecViaIDFromProducts Ps2 (rename_fid (getFdecID f1)) with
-  | None => false
-  | Some f2 => tv_fdec f1 f2 && tv_products Ps1' Ps2 
-  end
-| product_fdef f1::Ps1' =>
-  match lookupFdefViaIDFromProducts Ps2 (rename_fid (getFdefID f1)) with
-  | None => false
-  | Some f2 => tv_fdef f1 f2 && tv_products Ps1' Ps2 
-  end
 end.
 
 Fixpoint mtv_products (Ps Ps2:products) : bool :=
@@ -1286,34 +1351,47 @@ match Ps2 with
 | _::Ps2' => mtv_products Ps Ps2'
 end.
 
-Definition tv_module (m1 m2:module) :=
-match (m1, m2) with
-| (module_intro los1 nts1 Ps1, module_intro los2 nts2 Ps2) =>
-  sumbool2bool _ _ (layouts_dec los1 los2) &&
-  sumbool2bool _ _ (namedts_dec nts1 nts2) &&
-  tv_products Ps1 Ps2
-end.
-
 Definition mtv_module (m2:module) :=
 match m2 with
 | module_intro los2 nts2 Ps2 => mtv_products Ps2 Ps2
 end.
 
-Fixpoint tv_system (S1 S2:system) :=
-match (S1, S2) with
-| (nil, nil) => true
-| (m1::S1', m2::S2') => tv_module m1 m2 && tv_system S1' S2'
-| _ => false
-end.
-
+(***********************************)
+(* tactic *)
 Ltac sumbool_simpl :=
   repeat
   match goal with
   | [ H:sumbool2bool _ _ _ = true |- _ ] => apply sumbool2bool_true in H
   | [ H:is_true(sumbool2bool _ _ _) |- _ ] => apply sumbool2bool_true in H
-  | [ H:tv_cmds _ _ = true |- _ ] => unfold is_true in H; apply sumbool2bool_true in H
-  | [ H:is_true(tv_cmds _ _) |- _ ] => unfold is_true in H; apply sumbool2bool_true in H
+  | [ H:eq_value _ _ = true |- _ ] => apply sumbool2bool_true in H
+  | [ H:tv_typ _ _ = true |- _ ] => apply sumbool2bool_true in H
+  | [ H:tv_align _ _ = true |- _ ] => apply sumbool2bool_true in H
+  | [ H:eq_sterm _ _ = true |- _ ] => apply sumbool2bool_true in H
+  | [ H:eq_smem _ _ = true |- _ ] => apply sumbool2bool_true in H
+  | [ H:eq_id _ _ = true |- _ ] => apply sumbool2bool_true in H
+  | [ H:eq_const _ _ = true |- _ ] => apply sumbool2bool_true in H
+  | [ H:eq_l _ _ = true |- _ ] => apply sumbool2bool_true in H
   end.
+
+Ltac sumbool_subst :=
+  repeat
+  match goal with
+  | [ H:sumbool2bool _ _ _ = true |- _ ] => apply sumbool2bool_true in H; subst
+  | [ H:is_true(sumbool2bool _ _ _) |- _ ] => apply sumbool2bool_true in H; subst
+  | [ H:eq_value _ _ = true |- _ ] => apply sumbool2bool_true in H; subst
+  | [ H:tv_typ _ _ = true |- _ ] => apply sumbool2bool_true in H; subst
+  | [ H:tv_align _ _ = true |- _ ] => apply sumbool2bool_true in H; subst
+  | [ H:eq_sterm _ _ = true |- _ ] => apply sumbool2bool_true in H; subst
+  | [ H:eq_smem _ _ = true |- _ ] => apply sumbool2bool_true in H; subst
+  | [ H:eq_id _ _ = true |- _ ] => apply sumbool2bool_true in H; subst
+  | [ H:eq_const _ _ = true |- _ ] => apply sumbool2bool_true in H; subst
+  | [ H:eq_l _ _ = true |- _ ] => apply sumbool2bool_true in H; subst
+  end.
+
+Tactic Notation "sumbool_subst" "in" hyp(H) :=
+  apply sumbool2bool_true in H.
+
+
 
 (*****************************)
 (*
